theories/monotone.v
@@ -293,23 +293,12 @@ Section monotone.
     - destruct l; try discriminate. done. 
   Qed.
 
-  Notation monotonicity_guarantees_region ρ w p φ :=
-    (match ρ with
-     | Temporary => if pwl p then future_pub_mono else future_priv_mono
-     | Permanent => future_priv_mono
-     | Revoked => λ (_ : prodO STS STS * Word → iProp Σ) (_ : Word), True
-     end φ w)%I.
-
-  Notation monotonicity_guarantees_decide ρ w p φ :=
-    (if decide (ρ = Temporary ∧ pwl p = true)
-     then future_pub_mono (Σ := Σ) φ w
-     else future_priv_mono φ w)%I.
-
   (*Lemma that allows switching between the two different formulations of monotonicity, to alleviate the effects of inconsistencies*)
   Lemma switch_monotonicity_formulation ρ w p φ:
       monotonicity_guarantees_region ρ w p φ  ↔
-             (ρ ≠ Revoked → monotonicity_guarantees_decide ρ w p φ).
+             (ρ ≠ Revoked → monotonicity_guarantees_decide (Σ := Σ) ρ w p φ).
   Proof.
+    unfold monotonicity_guarantees_region, monotonicity_guarantees_decide.
     split.
     - destruct ρ.
       * destruct (pwl p) ; intros.
@@ -345,6 +334,7 @@ Lemma interp_monotone_generalW (W : WORLD)  (ρ : region_type) (p p0 p1 : Perm) 
   ((fixpoint interp1) W) (inr (p0, l, a2, a1, a0)) -∗
   monotonicity_guarantees_region ρ  (inr (p, g, b, e, a)) p1  (λne Wv : prodO (leibnizO (STS * STS)) (leibnizO Word), (interp Wv.1) Wv.2).
 Proof.
+  unfold monotonicity_guarantees_region.
   iIntros (Hstd Hwb Hfl' Hconds) "#Hvdst".
   destruct ρ.
   - destruct (pwl p1) eqn: HpwlP1 ; iAlways; simpl.
@@ -375,6 +365,7 @@ Lemma interp_monotone_generalZ (W : WORLD)  (ρ : region_type) (p0 p1 : Perm) (l
   ((fixpoint interp1) W) (inr (p0, l, a2, a1, a0)) -∗
   monotonicity_guarantees_region ρ  (inl z) p1  (λne Wv : prodO (leibnizO (STS * STS)) (leibnizO Word), (interp Wv.1) Wv.2).
 Proof.
+  unfold monotonicity_guarantees_region.
   iIntros (Hstd Hwb Hfl') "#Hvdst".
   destruct ρ.
   - destruct (pwl p1) eqn: HpwlP1 ; iAlways; simpl.
